theories/adequacy.v
@@ -11,35 +11,38 @@ Proof.
   econstructor 4; eauto.
 Qed.
 
-Lemma sim_adequacy (cfg_src cfg_tgt: expr * state)
+Lemma sim_adequacy {A: Type} Φ (sim_mem: A → state → state → Prop)
+  (σG: A) (cfg_src cfg_tgt: expr * state)
   (WFS: Wf cfg_src.2) (WFT: Wf cfg_tgt.2)
+  (SIM0: sim_state sim_mem σG cfg_src.2 cfg_tgt.2)
   (NO_UB: ∀ cfg', cfg_src ~t~>* cfg' → ¬ stuck cfg'.1 cfg'.2)
-  (SIM: sim (* (sim_terminal (λ _ _, True)) *) cfg_src cfg_tgt) :
+  (SIM: @sim A Φ sim_mem σG cfg_src cfg_tgt) :
   behaviors tstep cfg_tgt <1= behaviors tstep cfg_src.
 Proof.
-  intros ov BEH. revert cfg_src WFS WFT NO_UB SIM.
+  intros ov BEH. revert σG cfg_src WFS WFT SIM0 NO_UB SIM.
   induction BEH as [cfg_tgt|cfg_tgt|cfg_tgt v|cfg_tgt cfg_tgt' ov STEP BEH IH];
-    intros cfg_src WFS WFT NO_UB SIM.
-  - punfold SIM. destruct (SIM WFS WFT) as (? & ? & TERM & ?); [naive_solver|].
-    destruct TERM as (eσ2 & TS & TERM' & VAL); [by eexists|].
+    intros σG cfg_src WFS WFT SIM0 NO_UB SIM.
+  - punfold SIM. destruct (SIM WFS WFT SIM0) as (? & ? & TERM & ?); [naive_solver|].
+    destruct TERM as (eσ2 & σG' & TS & TERM' & VAL); [by eexists|].
     apply (rtc_step_behavior _ _ _ _ TS).
     constructor. by apply VAL.
-  - punfold SIM. destruct (SIM WFS WFT) as (SU & DIV & ?); [naive_solver|].
-    destruct SU as [eσ2 [TS' [IN NR]]].
+  - punfold SIM. destruct (SIM WFS WFT SIM0) as (SU & DIV & ?); [naive_solver|].
+    destruct SU as (eσ2 & TS' & IN & NR).
     + split; [by apply expr_terminal_False|].
       intros ???? PRIM. eapply (NS (e', σ')). econstructor; eauto.
     + apply (rtc_step_behavior _ _ _ _ TS').
       constructor 2; [by apply expr_terminal_False|].
       intros ? RED. inversion RED. by apply (NR _ _ _ _ PRIM).
-  - punfold SIM. destruct (SIM WFS WFT) as (SU & DIV & ?); [naive_solver|].
+  - punfold SIM. destruct (SIM WFS WFT SIM0) as (SU & DIV & ?); [naive_solver|].
     constructor. by apply DIV.
   - punfold SIM.
-    destruct (SIM WFS WFT) as (SU & DIV & TERM & TS); [naive_solver|].
-    destruct (TS cfg_tgt' STEP) as (eσ & STEP' & TS').
+    destruct (SIM WFS WFT SIM0) as (SU & DIV & TERM & TS); [naive_solver|].
+    destruct (TS cfg_tgt' STEP) as (eσ & σG' & STEP' & SS & HΦ & TS').
     eapply rtc_step_behavior; first by apply STEP'.
-    apply IH; simpl.
+    eapply IH; simpl.
     + by apply (rtc_tstep_wf _ _ STEP').
     + by apply (tstep_wf _ _ STEP).
+    + eauto.
     + intros cfg' S'. apply NO_UB. by etrans.
     + by inversion TS'.
 Qed.
